zoo/program_logic/structural_equality: Implement and verify [structeq].

theories/zoo/program_logic/structural_equality.v
@@ -12,11 +12,57 @@ From zoo Require Import
   options.
 
 Implicit Types b : bool.
+Implicit Types tag : nat.
 Implicit Types n : Z.
-Implicit Types v : val.
+Implicit Types l : location.
+Implicit Types gen : generativity.
+Implicit Types v w : val.
+Implicit Types vs : list val.
 Implicit Types lv : lowval.
 
-Parameter structeq : val.
+#[local] Definition __zoo_recs := (
+  recs: "structeq" "v1" "v2" =>
+    if: IsImmediate "v1" then
+      if: IsImmediate "v2" then
+        "v1" == "v2"
+      else
+        #false
+    else if: IsImmediate "v2" then
+      #false
+    else (
+      GetTag "v1" == GetTag "v2" and
+      let: "sz" := GetSize "v1" in
+      "sz" == GetSize "v2" and
+      "structeq_aux" "v1" "v2" "sz"
+    )
+  and: "structeq_aux" "v1" "v2" "i" =>
+    if: "i" == #0 then
+      #true
+    else
+      let: "i" := "i" - #1 in
+      "structeq" (Load "v1" "i" ) (Load "v2" "i") and
+      "structeq_aux" "v1" "v2" "i"
+)%zoo_recs.
+Definition structeq :=
+  ValRecs 0 __zoo_recs.
+#[local] Definition structeq_aux :=
+  ValRecs 1 __zoo_recs.
+#[global] Instance :
+  AsValRecs' structeq 0 __zoo_recs [
+    structeq ;
+    structeq_aux
+  ].
+Proof.
+  done.
+Qed.
+#[global] Instance :
+  AsValRecs' structeq_aux 1 __zoo_recs [
+    structeq ;
+    structeq_aux
+  ].
+Proof.
+  done.
+Qed.
 
 Notation "e1 = e2" := (
   App (App (Val structeq) e1%E) e2%E
@@ -70,31 +116,148 @@ Fixpoint val_traversable footprint v :=
   end.
 #[global] Arguments val_traversable _ !_ / : assert.
 
-Definition structeq_footprint `{zoo_G : !ZooG Σ} footprint : iProp Σ :=
-  [∗ map] l ↦ blk ∈ footprint,
-    l ↦ₕ Header blk.(structeq_block_tag) (length blk.(structeq_block_fields)) ∗
-    [∗ list] i ↦ fld ∈ blk.(structeq_block_fields),
-      (l +ₗ i) ↦{fld.(structeq_field_dfrac)} fld.(structeq_field_val) ∗
-      ⌜val_traversable footprint fld.(structeq_field_val)⌝.
+Section zoo_G.
+  Context `{zoo_G : !ZooG Σ}.
 
-Lemma structeq_footprint_empty `{zoo_G : !ZooG Σ} :
-  ⊢ structeq_footprint ∅.
-Proof.
-  setoid_rewrite big_sepM_empty. done.
-Qed.
+  Definition structeq_footprint footprint : iProp Σ :=
+    [∗ map] l ↦ blk ∈ footprint,
+      l ↦ₕ Header blk.(structeq_block_tag) (length blk.(structeq_block_fields)) ∗
+      [∗ list] i ↦ fld ∈ blk.(structeq_block_fields),
+        (l +ₗ i) ↦{fld.(structeq_field_dfrac)} fld.(structeq_field_val) ∗
+        ⌜val_traversable footprint fld.(structeq_field_val)⌝.
+
+  Lemma structeq_footprint_empty :
+    ⊢ structeq_footprint ∅.
+  Proof.
+    rewrite /structeq_footprint big_sepM_empty //.
+  Qed.
+
+  Lemma structeq_footprint_header {footprint} l blk :
+    footprint !! l = Some blk →
+    structeq_footprint footprint ⊢
+    l ↦ₕ Header blk.(structeq_block_tag) (length blk.(structeq_block_fields)).
+  Proof.
+    iIntros "%Hlookup Hfootprint".
+    iDestruct (big_sepM_lookup with "Hfootprint") as "($ & _)"; first done.
+  Qed.
+
+  Lemma structeq_footprint_lookup {footprint} l blk (i : nat) fld :
+    footprint !! l = Some blk →
+    blk.(structeq_block_fields) !! i = Some fld →
+    structeq_footprint footprint ⊢
+      (l +ₗ i) ↦{fld.(structeq_field_dfrac)} fld.(structeq_field_val) ∗
+      ⌜val_traversable footprint fld.(structeq_field_val)⌝ ∗
+      ( (l +ₗ i) ↦{fld.(structeq_field_dfrac)} fld.(structeq_field_val) -∗
+        structeq_footprint footprint
+      ).
+  Proof.
+    iIntros "%Hfootprint_lookup %Hfields_lookup Hfootprint".
+    iDestruct (big_sepM_lookup_acc with "Hfootprint") as "((#Hl_header & Hblk) & Hfootprint)"; first done.
+    iDestruct (big_sepL_lookup_acc with "Hblk") as "(HHfld & Hblk)"; first done.
+    iSteps.
+  Qed.
+  Lemma structeq_footprint_lookup' {footprint} l blk i :
+    footprint !! l = Some blk →
+    i < length blk.(structeq_block_fields) →
+    structeq_footprint footprint ⊢
+      ∃ fld,
+      ⌜blk.(structeq_block_fields) !! i = Some fld⌝ ∗
+      (l +ₗ i) ↦{fld.(structeq_field_dfrac)} fld.(structeq_field_val) ∗
+      ⌜val_traversable footprint fld.(structeq_field_val)⌝ ∗
+      ( (l +ₗ i) ↦{fld.(structeq_field_dfrac)} fld.(structeq_field_val) -∗
+        structeq_footprint footprint
+      ).
+  Proof.
+    iIntros "%Hfootprint_lookup %Hi Hfootprint".
+    destruct (lookup_lt_is_Some_2 blk.(structeq_block_fields) i) as (fld & Hfields_lookup); first done.
+    iExists fld. iStep.
+    iApply (structeq_footprint_lookup with "Hfootprint"); done.
+  Qed.
+
+  Lemma structeq_footprint_wp_tag {footprint} l blk :
+    footprint !! l = Some blk →
+    {{{
+      structeq_footprint footprint
+    }}}
+      GetTag #l
+    {{{
+      RET #(encode_tag blk.(structeq_block_tag));
+      structeq_footprint footprint
+    }}}.
+  Proof.
+    iIntros "%Hlookup %Φ Hfootprint HΦ".
+
+    iDestruct (structeq_footprint_header with "Hfootprint") as "#Hl_header"; first done.
+    iSteps.
+  Qed.
+  Lemma structeq_footprint_wp_size {footprint} l blk :
+    footprint !! l = Some blk →
+    {{{
+      structeq_footprint footprint
+    }}}
+      GetSize #l
+    {{{
+      RET #(length blk.(structeq_block_fields));
+      structeq_footprint footprint
+    }}}.
+  Proof.
+    iIntros "%Hlookup %Φ Hfootprint HΦ".
+
+    iDestruct (structeq_footprint_header with "Hfootprint") as "#Hl_header"; first done.
+    iSteps.
+  Qed.
+
+  Lemma structeq_footprint_wp_load {footprint} l blk (i : nat) fld :
+    footprint !! l = Some blk →
+    blk.(structeq_block_fields) !! i = Some fld →
+    {{{
+      structeq_footprint footprint
+    }}}
+      Load #l #i
+    {{{
+      RET fld.(structeq_field_val);
+      ⌜val_traversable footprint fld.(structeq_field_val)⌝ ∗
+      structeq_footprint footprint
+    }}}.
+  Proof.
+    iIntros "%Hfootprint_lookup %Hfields_lookup %Φ Hfootprint HΦ".
+
+    iDestruct (structeq_footprint_lookup with "Hfootprint") as "(Hl & %Htraversable & Hfootprint)"; [done.. |].
+    iSteps.
+  Qed.
+  Lemma structeq_footprint_wp_load' {footprint} l blk i :
+    footprint !! l = Some blk →
+    i < length blk.(structeq_block_fields) →
+    {{{
+      structeq_footprint footprint
+    }}}
+      Load #l #i
+    {{{ fld,
+      RET fld.(structeq_field_val);
+      ⌜blk.(structeq_block_fields) !! i = Some fld⌝ ∗
+      ⌜val_traversable footprint fld.(structeq_field_val)⌝ ∗
+      structeq_footprint footprint
+    }}}.
+  Proof.
+    iIntros "%Hfootprint_lookup %Hi %Φ Hfootprint HΦ".
+
+    iDestruct (structeq_footprint_lookup' with "Hfootprint") as "(%fld & %Hfields_lookup & Hl & %Htraversable & Hfootprint)"; [done.. |].
+    iSteps.
+  Qed.
+End zoo_G.
 
 Fixpoint val_reachable footprint src path dst :=
   match path with
   | [] =>
       src = dst
-  | pos :: path =>
+  | i :: path =>
       match src with
       | ValLoc l =>
           match footprint !! l with
           | None =>
               False
           | Some blk =>
-              match blk.(structeq_block_fields) !! pos with
+              match blk.(structeq_block_fields) !! i with
               | None =>
                   False
               | Some fld =>
@@ -102,7 +265,7 @@ Fixpoint val_reachable footprint src path dst :=
               end
           end
       | ValBlock _ _ vs =>
-          match vs !! pos with
+          match vs !! i with
           | None =>
               False
           | Some src =>
@@ -123,27 +286,27 @@ Proof.
       match path with
       | [] =>
           cast_if (decide (src = dst))
-      | pos :: path =>
+      | i :: path =>
           match src with
           | ValLoc l =>
               (match footprint !! l as x return _ = x → _ with
               | None => λ Hfootprint_lookup,
                   right _
               | Some blk => λ Hfootprint_lookup,
-                  (match blk.(structeq_block_fields) !! pos as x return _ = x → _ with
+                  (match blk.(structeq_block_fields) !! i as x return _ = x → _ with
                   | None => λ Hfields_lookup,
                       right _
                   | Some fld => λ Hfields_lookup,
                       cast_if (go fld.(structeq_field_val) path)
-                  end) (eq_refl (blk.(structeq_block_fields) !! pos))
+                  end) (eq_refl (blk.(structeq_block_fields) !! i))
               end) (eq_refl (footprint !! l))
           | ValBlock _ _ vs =>
-              (match vs !! pos as x return _ = x → _ with
+              (match vs !! i as x return _ = x → _ with
               | None => λ Hvs_lookup,
                   right _
               | Some src => λ Hvs_lookup,
                   cast_if (go src path)
-              end) (eq_refl (vs !! pos))
+              end) (eq_refl (vs !! i))
           | _ =>
               right _
           end
@@ -209,18 +372,473 @@ Definition val_structneq footprint v1 v2 :=
   val_reachable footprint v2 path v2' ∧
   val_compatible footprint v1' v2' = false.
 
-Axiom structeq_spec : ∀ `{zoo_G : !ZooG Σ} {v1 v2} footprint,
-  val_traversable footprint v1 →
-  val_traversable footprint v2 →
-  {{{
-    structeq_footprint footprint
-  }}}
-    v1 = v2
-  {{{ b,
-    RET #b;
-    ⌜(if b then val_structeq else val_structneq) footprint v1 v2⌝ ∗
-    structeq_footprint footprint
-  }}}.
+Lemma val_immediate_structeq footprint v1 v2 :
+  val_immediate v1 →
+  val_immediate v2 →
+  v1 ≈ v2 →
+  val_structeq footprint v1 v2.
+Proof.
+  intros Himmediate1 Himmediate2 Hsimilar.
+  intros path v1_ v2_ Hreachable1 Hreachable2.
+  destruct v1 as [[b1 | n1 | l1 | |] | | gen1 tag1 []]; try done.
+  all: destruct v2 as [[b2 | n2 | l2 | |] | | gen2 tag2 []]; try done.
+  all: destruct path; last done.
+  all: simplify.
+  all: cbn.
+  all: rewrite bool_decide_eq_true_2 //.
+Qed.
+Lemma val_immediate_structneq footprint v1 v2 :
+  val_immediate v1 →
+  val_immediate v2 →
+  v1 ≉ v2 →
+  val_structneq footprint v1 v2.
+Proof.
+  intros Himmediate1 Himmediate2 Hnonsimilar.
+  eexists [], v1, v2. split_and!; try done.
+  destruct v1 as [[b1 | n1 | l1 | |] | | gen1 tag1 []]; try done.
+  all: destruct v2 as [[b2 | n2 | l2 | |] | | gen2 tag2 []]; try done.
+  all: cbn.
+  all: rewrite bool_decide_eq_false_2 //.
+  all: naive_solver.
+Qed.
+
+Lemma val_structeq_refl footprint v :
+  val_immediate v →
+  val_structeq footprint v v.
+Proof.
+  intros Himmediate.
+  apply val_immediate_structeq; done.
+Qed.
+Lemma val_structeq_refl' footprint v1 v2 :
+  v1 = v2 →
+  val_immediate v1 →
+  val_structeq footprint v1 v2.
+Proof.
+  intros ->.
+  apply val_structeq_refl.
+Qed.
+
+Section zoo_G.
+  Context `{zoo_G : !ZooG Σ}.
+
+  #[local] Lemma structeq_spec_aux :
+    ⊢ (
+      ∀ v1 v2 footprint,
+      {{{
+        ⌜val_traversable footprint v1⌝ ∗
+        ⌜val_traversable footprint v2⌝ ∗
+        structeq_footprint footprint
+      }}}
+        v1 = v2
+      {{{ b,
+        RET #b;
+        ⌜(if b then val_structeq else val_structneq) footprint v1 v2⌝ ∗
+        structeq_footprint footprint
+      }}}
+    ) ∧ (
+      ∀ l1 blk1 l2 blk2 footprint i,
+      {{{
+        ⌜0 ≤ i ≤ length blk1.(structeq_block_fields)⌝%Z ∗
+        ⌜footprint !! l1 = Some blk1⌝ ∗
+        ⌜footprint !! l2 = Some blk2⌝ ∗
+        ⌜blk1.(structeq_block_tag) = blk2.(structeq_block_tag)⌝ ∗
+        ⌜length blk1.(structeq_block_fields) = length blk2.(structeq_block_fields)⌝ ∗
+        structeq_footprint footprint ∗
+        ⌜ ∀ j fld1 fld2,
+          blk1.(structeq_block_fields) !! j = Some fld1 →
+          blk2.(structeq_block_fields) !! j = Some fld2 →
+          ₊i ≤ j →
+          val_structeq footprint fld1.(structeq_field_val) fld2.(structeq_field_val)
+        ⌝
+      }}}
+        structeq_aux #l1 #l2 #i
+      {{{ b,
+        RET #b;
+        ⌜(if b then val_structeq else val_structneq) footprint #l1 #l2⌝ ∗
+        structeq_footprint footprint
+      }}}
+    ) ∧ (
+      ∀ l1 blk1 gen2 tag2 vs2 footprint i,
+      let v2 := ValBlock gen2 tag2 vs2 in
+      {{{
+        ⌜0 ≤ i ≤ length vs2⌝%Z ∗
+        ⌜footprint !! l1 = Some blk1⌝ ∗
+        ⌜blk1.(structeq_block_tag) = tag2⌝ ∗
+        ⌜length blk1.(structeq_block_fields) = length vs2⌝ ∗
+        ⌜0 < length vs2⌝ ∗
+        ⌜val_traversable footprint v2⌝ ∗
+        structeq_footprint footprint ∗
+        ⌜ ∀ j fld1 v2,
+          blk1.(structeq_block_fields) !! j = Some fld1 →
+          vs2 !! j = Some v2 →
+          ₊i ≤ j →
+          val_structeq footprint fld1.(structeq_field_val) v2
+        ⌝
+      }}}
+        structeq_aux #l1 v2 #i
+      {{{ b,
+        RET #b;
+        ⌜(if b then val_structeq else val_structneq) footprint #l1 v2⌝ ∗
+        structeq_footprint footprint
+      }}}
+    ) ∧ (
+      ∀ gen1 tag1 vs1 l2 blk2 footprint i,
+      let v1 := ValBlock gen1 tag1 vs1 in
+      {{{
+        ⌜0 ≤ i ≤ length vs1⌝%Z ∗
+        ⌜footprint !! l2 = Some blk2⌝ ∗
+        ⌜tag1 = blk2.(structeq_block_tag)⌝ ∗
+        ⌜length vs1 = length blk2.(structeq_block_fields)⌝ ∗
+        ⌜0 < length vs1⌝ ∗
+        ⌜val_traversable footprint v1⌝ ∗
+        structeq_footprint footprint ∗
+        ⌜ ∀ j v1 fld2,
+          vs1 !! j = Some v1 →
+          blk2.(structeq_block_fields) !! j = Some fld2 →
+          ₊i ≤ j →
+          val_structeq footprint v1 fld2.(structeq_field_val)
+        ⌝
+      }}}
+        structeq_aux v1 #l2 #i
+      {{{ b,
+        RET #b;
+        ⌜(if b then val_structeq else val_structneq) footprint v1 #l2⌝ ∗
+        structeq_footprint footprint
+      }}}
+    ) ∧ (
+      ∀ gen1 tag1 vs1 gen2 tag2 vs2 footprint i,
+      let v1 := ValBlock gen1 tag1 vs1 in
+      let v2 := ValBlock gen2 tag2 vs2 in
+      {{{
+        ⌜0 ≤ i ≤ length vs1⌝%Z ∗
+        ⌜tag1 = tag2⌝ ∗
+        ⌜length vs1 = length vs2⌝ ∗
+        ⌜0 < length vs1⌝ ∗
+        ⌜val_traversable footprint v1⌝ ∗
+        ⌜val_traversable footprint v2⌝ ∗
+        structeq_footprint footprint ∗
+        ⌜ ∀ j v1 v2,
+          vs1 !! j = Some v1 →
+          vs2 !! j = Some v2 →
+          ₊i ≤ j →
+          val_structeq footprint v1 v2
+        ⌝
+      }}}
+        structeq_aux v1 v2 #i
+      {{{ b,
+        RET #b;
+        ⌜(if b then val_structeq else val_structneq) footprint v1 v2⌝ ∗
+        structeq_footprint footprint
+      }}}
+    ).
+  Proof.
+    iLöb as "HLöb".
+    iDestruct "HLöb" as "(IHstructeq & IHstructeq_aux_loc_loc & IHstructeq_aux_loc_block & IHstructeq_aux_block_loc & IHstructeq_aux_block_block)".
+    repeat iSplit.
+
+    { iClear "IHstructeq".
+      iIntros "%v1 %v2 %footprint !> %Φ (%Htraversable1 & %Htraversable2 & Hfootprint) HΦ".
+
+      wp_recs. wp_pures.
+
+      all: destruct v1 as [[b1 | n1 | l1 | |] | | gen1 tag1 [| v1 vs1]].
+      all: try done.
+      all: wp_pures.
+
+      all: destruct v2 as [[b2 | n2 | l2 | |] | | gen2 tag2 [| v2 vs2]].
+      all: try done.
+      all: wp_pures.
+
+      all:
+        try match goal with |- _ _ (WP _ == _ {{ _ }})%I =>
+          wp_apply wp_equal_nobranch as (b) "%Hb"
+        end.
+      all:
+        try match goal with |- _ _ ?P =>
+          tryif eunify P (wp _ _ _ _) then idtac else
+            iStepFrameSteps
+        end.
+      all:
+        try (
+          iPureIntro;
+          try (eexists [], _, _; done);
+          try (
+            destruct b; cbn in Hb;
+            [ apply val_immediate_structeq; done
+            | apply val_immediate_structneq; done
+            ]
+          );
+          try (
+            case_bool_decide;
+            [ apply val_structeq_refl'; naive_solver
+            | apply val_immediate_structneq; [done.. |];
+              cbn; naive_solver
+            ]
+          )
+        ).
+
+      - apply elem_of_dom in Htraversable1 as (blk1 & Hfootprint_lookup_1).
+        apply elem_of_dom in Htraversable2 as (blk2 & Hfootprint_lookup_2).
+        wp_apply (structeq_footprint_wp_tag with "Hfootprint") as "Hfootprint"; first done.
+        wp_apply (structeq_footprint_wp_tag with "Hfootprint") as "Hfootprint"; first done.
+        wp_pures.
+        case_bool_decide; wp_pures.
+        + wp_apply (structeq_footprint_wp_size with "Hfootprint") as "Hfootprint"; first done.
+          wp_smart_apply (structeq_footprint_wp_size with "Hfootprint") as "Hfootprint"; first done.
+          wp_pures.
+          case_bool_decide; wp_pures.
+          * wp_apply ("IHstructeq_aux_loc_loc" with "[$Hfootprint] HΦ").
+            iPureIntro. split_and!; [naive_solver lia.. |].
+            intros j ? ? ? Hj%lookup_lt_Some. lia.
+          * iSteps. iPureIntro.
+            eexists [], _, _. split_and!; try done.
+            cbn. erewrite !lookup_total_correct; [| done..].
+            rewrite andb_false_iff !beq_spec'. naive_solver.
+        + iSteps. iPureIntro.
+          eexists [], _, _. split_and!; try done.
+          cbn. erewrite !lookup_total_correct; [| done..].
+          rewrite andb_false_iff !beq_spec'. naive_solver.
+
+      - apply elem_of_dom in Htraversable1 as (blk1 & Hfootprint_lookup_1).
+        wp_apply (structeq_footprint_wp_tag with "Hfootprint") as "Hfootprint"; first done.
+        wp_pures.
+        case_bool_decide; wp_pures.
+        + wp_apply (structeq_footprint_wp_size with "Hfootprint") as "Hfootprint"; first done.
+          wp_pures.
+          case_bool_decide; wp_pures.
+          * wp_apply ("IHstructeq_aux_loc_block" with "[$Hfootprint] HΦ").
+            iPureIntro. split_and!; [naive_solver lia.. |].
+            intros j ? ? ? Hj%lookup_lt_Some. simpl in Hj. lia.
+          * iSteps. iPureIntro.
+            eexists [], _, _. split_and!; try done.
+            cbn. erewrite !lookup_total_correct; [| done..].
+            rewrite andb_false_iff !beq_spec'. naive_solver.
+        + iSteps. iPureIntro.
+          eexists [], _, _. split_and!; try done.
+          cbn. erewrite !lookup_total_correct; [| done..].
+          rewrite andb_false_iff !beq_spec'. naive_solver.
+
+      - apply elem_of_dom in Htraversable2 as (blk2 & Hfootprint_lookup_2).
+        wp_apply (structeq_footprint_wp_tag with "Hfootprint") as "Hfootprint"; first done.
+        wp_pures.
+        case_bool_decide; wp_pures.
+        + wp_apply (structeq_footprint_wp_size with "Hfootprint") as "Hfootprint"; first done.
+          wp_pures.
+          case_bool_decide; wp_pures.
+          * wp_apply ("IHstructeq_aux_block_loc" with "[$Hfootprint] HΦ").
+            iPureIntro. split_and!; [naive_solver lia.. |].
+            intros j ? ? ? Hj%lookup_lt_Some. lia.
+          * iSteps. iPureIntro.
+            eexists [], _, _. split_and!; try done.
+            cbn. erewrite !lookup_total_correct; [| done..].
+            rewrite andb_false_iff !beq_spec'. naive_solver.
+        + iSteps. iPureIntro.
+          eexists [], _, _. split_and!; try done.
+          cbn. erewrite !lookup_total_correct; [| done..].
+          rewrite andb_false_iff !beq_spec'. naive_solver.
+
+      - case_bool_decide; wp_pures.
+        + case_bool_decide; wp_pures.
+          * wp_apply ("IHstructeq_aux_block_block" with "[$Hfootprint] HΦ").
+            iPureIntro. split_and!; [naive_solver lia.. |].
+            intros j ? ? ? Hj%lookup_lt_Some. simpl in Hj. lia.
+          * iSteps. iPureIntro.
+            eexists [], _, _. split_and!; try done.
+            rewrite andb_false_iff !beq_spec'. naive_solver.
+        + iSteps. iPureIntro.
+          eexists [], _, _. split_and!; try done.
+          rewrite andb_false_iff !beq_spec'. naive_solver.
+    }
+
+    { iClear "IHstructeq_aux_loc_block IHstructeq_aux_block_loc IHstructeq_aux_block_block".
+      iIntros "%l1 %blk1 %l2 %blk2 %footprint %i !> %Φ (%Hi & %Hfootprint_lookup_1 & %Hfootprint_lookup_2 & % & % & Hfootprint & %Hstructeq) HΦ".
+
+      wp_recs. wp_pures.
+      case_bool_decide; wp_pures.
+
+      - iSteps. iPureIntro.
+        intros [| j path] dst1 dst2 Hreachable1 Hreachable2.
+        all: simplify.
+
+        + rewrite andb_true_iff !beq_spec.
+          erewrite !lookup_total_correct; done.
+
+        + rewrite Hfootprint_lookup_1 in Hreachable1.
+          destruct (blk1.(structeq_block_fields) !! j) as [fld1 |] eqn:Hfields1_lookup; last done.
+          rewrite Hfootprint_lookup_2 in Hreachable2.
+          destruct (blk2.(structeq_block_fields) !! j) as [fld2 |] eqn:Hfields2_lookup; last done.
+          eapply Hstructeq; done || lia.
+
+      - replace (i - 1)%Z with ⁺(₊i - 1) by lia.
+
+        wp_apply (structeq_footprint_wp_load' with "Hfootprint") as (fld2) "(%Hfields2_lookup & %Htraversable2 & Hfootprint)"; [done | lia |].
+        wp_apply (structeq_footprint_wp_load' with "Hfootprint") as (fld1) "(%Hfields1_lookup & %Htraversable1 & Hfootprint)"; [done | lia |].
+        wp_smart_apply ("IHstructeq" with "[$Hfootprint]") as (b) "(%Hb & Hfootprint)"; first iSteps.
+        destruct b; wp_pures.
+
+        + wp_apply ("IHstructeq_aux_loc_loc" with "[$Hfootprint] HΦ").
+          iPureIntro. split_and!; try done; try lia.
+          intros j.
+          destruct_decide (j = ₊i - 1); naive_solver lia.
+
+        + iSteps. iPureIntro.
+          destruct Hb as (path & w1 & w2 & Hreachable1 & Hreachable2 & Hcompatible).
+          eexists (₊i - 1 :: path), w1, w2. split_and!; last done.
+          * rewrite /= Hfootprint_lookup_1 Hfields1_lookup //.
+          * rewrite /= Hfootprint_lookup_2 Hfields2_lookup //.
+    }
+
+    { iClear "IHstructeq_aux_loc_loc IHstructeq_aux_block_loc IHstructeq_aux_block_block".
+      iIntros "%l1 %blk1 %gen2 %tag2 %vs2 %footprint %i !> %Φ (%Hi & %Hfootprint_lookup_1 & % & % & % & %Htraversable2 & Hfootprint & %Hstructeq) HΦ".
+
+      wp_recs. wp_pures.
+      case_bool_decide; wp_pures.
+
+      - iSteps. iPureIntro.
+        intros [| j path] dst1 dst2 Hreachable1 Hreachable2.
+        all: simplify.
+
+        + destruct vs2 as [| v2 vs2]; first naive_solver lia.
+          rewrite andb_true_iff !beq_spec.
+          erewrite !lookup_total_correct; done.
+
+        + rewrite Hfootprint_lookup_1 in Hreachable1.
+          destruct (blk1.(structeq_block_fields) !! j) as [fld1 |] eqn:Hfields1_lookup; last done.
+          destruct (vs2 !! j) as [v2 |] eqn:Hvs2_lookup; last done.
+          eapply Hstructeq; done || lia.
+
+      - replace (i - 1)%Z with ⁺(₊i - 1) by lia.
+
+        destruct (lookup_lt_is_Some_2 vs2 (₊i - 1)) as (v2 & Hvs2_lookup); first lia.
+
+        wp_pures.
+        wp_apply (structeq_footprint_wp_load' with "Hfootprint") as (fld1) "(%Hfields1_lookup & %Htraversable1 & Hfootprint)"; [done | lia |].
+        wp_smart_apply ("IHstructeq" with "[$Hfootprint]") as (b) "(%Hb & Hfootprint)"; first iSteps.
+        { iPureIntro.
+          rewrite /= Forall'_Forall Forall_lookup in Htraversable2.
+          naive_solver.
+        }
+        destruct b; wp_pures.
+
+        + wp_apply ("IHstructeq_aux_loc_block" with "[$Hfootprint] HΦ").
+          iPureIntro. split_and!; try done; try lia.
+          intros j.
+          destruct_decide (j = ₊i - 1); naive_solver lia.
+
+        + iSteps. iPureIntro.
+          destruct Hb as (path & w1 & w2 & Hreachable1 & Hreachable2 & Hcompatible).
+          eexists (₊i - 1 :: path), w1, w2. split_and!; last done.
+          * rewrite /= Hfootprint_lookup_1 Hfields1_lookup //.
+          * rewrite /= Hvs2_lookup //.
+    }
+
+    { iClear "IHstructeq_aux_loc_loc IHstructeq_aux_loc_block IHstructeq_aux_block_block".
+      iIntros "%gen1 %tag1 %vs1 %l2 %blk2 %footprint %i !> %Φ (%Hi & %Hfootprint_lookup_2 & % & % & % & %Htraversable1 & Hfootprint & %Hstructeq) HΦ".
+
+      wp_recs. wp_pures.
+      case_bool_decide; wp_pures.
+
+      - iSteps. iPureIntro.
+        intros [| j path] dst1 dst2 Hreachable1 Hreachable2.
+        all: simplify.
+
+        + destruct vs1 as [| v1 vs1]; first naive_solver lia.
+          rewrite andb_true_iff !beq_spec.
+          erewrite !lookup_total_correct; done.
+
+        + destruct (vs1 !! j) as [v1 |] eqn:Hvs1_lookup; last done.
+          rewrite Hfootprint_lookup_2 in Hreachable2.
+          destruct (blk2.(structeq_block_fields) !! j) as [fld2 |] eqn:Hfields2_lookup; last done.
+          eapply Hstructeq; done || lia.
+
+      - replace (i - 1)%Z with ⁺(₊i - 1) by lia.
+
+        destruct (lookup_lt_is_Some_2 vs1 (₊i - 1)) as (v1 & Hvs1_lookup); first lia.
+
+        wp_pures.
+        wp_apply (structeq_footprint_wp_load' with "Hfootprint") as (fld2) "(%Hfields2_lookup & %Htraversable2 & Hfootprint)"; [done | lia |].
+        wp_smart_apply ("IHstructeq" with "[$Hfootprint]") as (b) "(%Hb & Hfootprint)"; first iSteps.
+        { iPureIntro.
+          rewrite /= Forall'_Forall Forall_lookup in Htraversable1.
+          naive_solver.
+        }
+        destruct b; wp_pures.
+
+        + wp_apply ("IHstructeq_aux_block_loc" with "[$Hfootprint] HΦ").
+          iPureIntro. split_and!; try done; try lia.
+          intros j.
+          destruct_decide (j = ₊i - 1); naive_solver lia.
+
+        + iSteps. iPureIntro.
+          destruct Hb as (path & w1 & w2 & Hreachable1 & Hreachable2 & Hcompatible).
+          eexists (₊i - 1 :: path), w1, w2. split_and!; last done.
+          * rewrite /= Hvs1_lookup //.
+          * rewrite /= Hfootprint_lookup_2 Hfields2_lookup //.
+    }
+
+    { iClear "IHstructeq_aux_loc_loc IHstructeq_aux_loc_block IHstructeq_aux_block_loc".
+      iIntros "%gen1 %tag1 %vs1 %gen2 %tag2 %vs2 %footprint %i !> %Φ (%Hi & -> & % & % & %Htraversable1 & %Htraversable2 & Hfootprint & %Hstructeq) HΦ".
+
+      wp_recs. wp_pures.
+      case_bool_decide; wp_pures.
+
+      - iSteps. iPureIntro.
+        intros [| j path] dst1 dst2 Hreachable1 Hreachable2.
+        all: simplify.
+
+        + destruct vs1 as [| v1 vs1]; first naive_solver lia.
+          destruct vs2 as [| v2 vs2]; first naive_solver lia.
+          rewrite andb_true_iff !beq_spec //.
+
+        + destruct (vs1 !! j) as [v1 |] eqn:Hvs1_lookup; last done.
+          destruct (vs2 !! j) as [v2 |] eqn:Hvs2_lookup; last done.
+          eapply Hstructeq; done || lia.
+
+      - replace (i - 1)%Z with ⁺(₊i - 1) by lia.
+
+        destruct (lookup_lt_is_Some_2 vs1 (₊i - 1)) as (v1 & Hvs1_lookup); first lia.
+        destruct (lookup_lt_is_Some_2 vs2 (₊i - 1)) as (v2 & Hvs2_lookup); first lia.
+
+        wp_pures.
+        wp_smart_apply ("IHstructeq" with "[$Hfootprint]") as (b) "(%Hb & Hfootprint)".
+        { iPureIntro.
+          rewrite /= !Forall'_Forall !Forall_lookup in Htraversable1 Htraversable2.
+          naive_solver.
+        }
+        destruct b; wp_pures.
+
+        + wp_apply ("IHstructeq_aux_block_block" with "[$Hfootprint] HΦ").
+          iPureIntro. split_and!; try done; try lia.
+          intros j.
+          destruct_decide (j = ₊i - 1); naive_solver lia.
+
+        + iSteps. iPureIntro.
+          destruct Hb as (path & w1 & w2 & Hreachable1 & Hreachable2 & Hcompatible).
+          eexists (₊i - 1 :: path), w1, w2. split_and!; last done.
+          * rewrite /= Hvs1_lookup //.
+          * rewrite /= Hvs2_lookup //.
+    }
+  Qed.
+  Lemma structeq_spec {v1 v2} footprint :
+    val_traversable footprint v1 →
+    val_traversable footprint v2 →
+    {{{
+      structeq_footprint footprint
+    }}}
+      v1 = v2
+    {{{ b,
+      RET #b;
+      ⌜(if b then val_structeq else val_structneq) footprint v1 v2⌝ ∗
+      structeq_footprint footprint
+    }}}.
+  Proof.
+    iIntros "%Htraversable1 %Htraversable2 %Φ Hfootprint HΦ".
+    iDestruct structeq_spec_aux as "(H & _)".
+    iApply ("H" with "[$Hfootprint]"); iSteps.
+  Qed.
+End zoo_G.
+
+#[global] Opaque structeq.
 
 (* Abstract (tree-like) values *)
 
